impl_proofs/replCorrectScript.sml
@@ -2,7 +2,7 @@ open preamble boolSimps miscLib rich_listTheory;
 open lexer_funTheory repl_funTheory replTheory untypedSafetyTheory bytecodeClockTheory bytecodeExtraTheory bytecodeEvalTheory
 open lexer_implTheory mmlParseTheory inferSoundTheory BigStepTheory ElabTheory compileLabelsTheory compilerProofsTheory;
 open SemanticPrimitivesTheory semanticsExtraTheory TypeSystemTheory typeSoundTheory weakeningTheory typeSysPropsTheory terminationTheory;
-open repl_fun_altTheory repl_fun_alt_proofTheory;
+open bootstrapProofsTheory repl_fun_altTheory repl_fun_alt_proofTheory;
 
 val _ = new_theory "replCorrect";
 
@@ -1514,19 +1514,6 @@ rw [init_env_def, initial_program_def, evaluate_dec_cases, LibTheory.emp_def, pm
 NTAC 15 (rw [Once evaluate_cases]) >>
 rw [do_con_check_def, AstTheory.pat_bindings_def, pmatch_def, LibTheory.bind_def]);
 
-val empty_env_rs = Q.prove (
-`(LENGTH bc.stack = 0) ∧ (bc.clock = SOME ck) ∧ (rd.cls = FEMPTY) ∧ (rd.sm = []) ⇒ 
- env_rs [] [] [] init_compiler_state (LENGTH bc.stack) rd (ck,[]) (bc with code := bc_inst_list)`,
-       rw [env_rs_def, CompilerTheory.init_compiler_state_def, LET_THM, good_contab_def, IntLangTheory.tuple_cn_def,
-           toIntLangProofsTheory.cmap_linv_def, intLangExtraTheory.good_cmap_def, cenv_dom_def, FLOOKUP_DEF] >>
-       qexists_tac `[]` >>
-       rw [pmatchTheory.env_to_Cenv_MAP, closed_Clocs_def, closed_vlabs_def, intLangExtraTheory.all_vlabs_menv_def,
-           intLangExtraTheory.vlabs_menv_def] >-
-       (* SO: Looks like a trivial suim I just don't know the magic for *)
-       cheat >>
-       rw [toBytecodeProofsTheory.Cenv_bs_def, toBytecodeProofsTheory.env_renv_def, toBytecodeProofsTheory.s_refs_def,
-           toBytecodeProofsTheory.good_rd_def, FEVERY_DEF]);
-
 val initial_invariant = prove(
   ``invariant init_repl_state initial_repl_fun_state initial_bc_state``,
   rw[invariant_def,initial_repl_fun_state_def,initial_elaborator_state_def,init_repl_state_def,LET_THM] >>
@@ -1545,29 +1532,59 @@ val initial_invariant = prove(
   `evaluate_top [] [] [] [] (Tdec initial_program) ([],[],Rval ([],init_env))` 
         by (rw [evaluate_top_cases, LibTheory.emp_def] >>
             metis_tac [eval_initial_program]) >>
-  imp_res_tac compile_top_thm >>
-  rw [] >>
-  fs [closed_top_def, closed_context_def, toIntLangProofsTheory.closed_under_cenv_def,
-      closed_under_menv_def] >>
+
+  qspecl_then[`[]`,`[]`,`[]`,`[]`,`Tdec initial_program`,`([],[],Rval ([],init_env))`]mp_tac compile_top_thm >>
+  simp[] >>
+  simp[closed_top_def,closed_context_def,toIntLangProofsTheory.closed_under_cenv_def,closed_under_menv_def] >>
   `FV_dec initial_program = {}`
           by (rw [initial_program_def, EXTENSION] >> metis_tac []) >>
   `dec_cns initial_program ⊆ cenv_dom ([]:envC)`
           by (rw [initial_program_def, cenv_dom_def, SUBSET_DEF]) >>
   fs [] >>
-  pop_assum (fn _ => all_tac) >>
-  pop_assum (fn _ => all_tac) >>
-  pop_assum (strip_assume_tac o Q.SPEC `init_compiler_state`) >>
-  pop_assum (strip_assume_tac o Q.SPECL [`FST compile_primitives`, 
-                                         `FST (SND compile_primitives)`, 
-                                         `UNKNOWN_rd`,
-                                         `SND (SND compile_primitives)`,
-                                         `initial_bc_state`,
-                                         `UNKNOWN_bc_inst_list`]) >>
-
-  (* env_rs stuff *)
-  (* want to get this from evaluating the initial program from empty and using
-  the normal invariant preservation theorem *)
-  cheat)
+  disch_then(qspec_then`init_compiler_state`mp_tac) >>
+  disch_then(qx_choosel_then[`ck`]mp_tac) >>
+  qabbrev_tac`p = compile_top init_compiler_state (Tdec initial_program)` >>
+  PairCases_on`p`>>simp[] >>
+  disch_then(qspecl_then
+    [`<|sm:=[];cls:=FEMPTY|>`
+    ,`^(rand(rhs(concl(initial_bc_state_def)))) with
+      <| pc := next_addr (K 0) [PrintE;Stop]
+       ; clock := SOME ck
+       ; code := [PrintE;Stop]++(REVERSE p2)|>`
+    ,`[PrintE;Stop]`]mp_tac) >>
+  discharge_hyps >- (
+    simp[] >>
+    simp[good_labels_def] >>
+    match_mp_tac env_rs_empty >>
+    simp[] ) >>
+  disch_then(qx_choosel_then[`bs`,`rd`]strip_assume_tac) >>
+  map_every qexists_tac[`rd`,`0`] >>
+  `FST compile_primitives = p0` by (
+    simp[compile_primitives_def] ) >>
+  imp_res_tac RTC_bc_next_can_be_unclocked >>
+  qpat_assum`bc_next^* X bs`kall_tac >>
+  imp_res_tac RTC_bc_next_bc_eval >>
+  pop_assum mp_tac >>
+  discharge_hyps >- (
+    simp[bc_eval1_thm] >>
+    `bc_fetch (bs with clock := NONE) = NONE` by (
+      simp[BytecodeTheory.bc_fetch_def,bc_fetch_with_clock] >>
+      match_mp_tac bc_fetch_aux_end_NONE >>
+      imp_res_tac RTC_bc_next_preserves >> fs[] >>
+      simp[SUM_REVERSE,FILTER_REVERSE,MAP_REVERSE] ) >>
+    simp[bc_eval1_def] ) >>
+  strip_tac >>
+  `bs with clock := NONE = initial_bc_state` by (
+    simp[initial_bc_state_def] >>
+    qmatch_assum_abbrev_tac`bc_eval bs0 = SOME bs1` >>
+    Q.PAT_ABBREV_TAC`bs0' = install_code x y z` >>
+    `bs0' = bs0` by (
+      simp[Abbr`bs0`,Abbr`bs0'`,install_code_def] >>
+      simp[bc_state_component_equality] >>
+      simp[compile_primitives_def]) >>
+    simp[]) >>
+  `(bs with clock := NONE).stack = bs.stack` by rw[] >>
+  metis_tac[env_rs_remove_clock,SND])
 
 val replCorrect = Q.store_thm ("replCorrect",
 `!input output.
